Update 2.reduction_independentSet_to_vertexCover.dfy

2.reduction_independentSet_to_vertexCover.dfy
@@ -1,7 +1,6 @@
 // Nodes in an undirected graph are natural numbers
 datatype Graph = G(V: set<nat>, E: set<(nat, nat)>)
 
-
 // The undirected graph is valid
 ghost predicate valid_graph(g: Graph)
 {
@@ -10,8 +9,7 @@ ghost predicate valid_graph(g: Graph)
 
 // Independent-Set decision problem.
 predicate indSet(g: Graph, k: nat)
-    requires valid_graph(g)
-    requires k <= |g.V|
+    requires valid_graph(g) && k <= |g.V|
 {
     exists ins: set<nat> :: |ins| == k && ins <= g.V && is_indSet(g, ins)
 }
@@ -25,18 +23,18 @@ predicate is_indSet(g: Graph, ins: set<nat>)
 
 
 // Vertex-Cover decision problem.
-ghost predicate vertexCover(g: Graph, k: nat)
-    requires valid_graph(g)
-    requires k <= |g.V|
+predicate vertexCover(g: Graph, k: nat)
+    requires valid_graph(g) && k <= |g.V|
 {
     exists vc: set<nat> :: |vc| == k && vc <= g.V && is_vertexCover(g, vc)
 }
 
-ghost predicate is_vertexCover(g: Graph, vc: set<nat>)
+predicate is_vertexCover(g: Graph, vc: set<nat>)
     requires valid_graph(g)
     requires vc <= g.V
 {
-    forall u: nat, v: nat :: (u, v) in g.E ==> (u in vc || v in vc) 
+    forall u: nat, v: nat :: u in g.V && v in g.V && (u, v) in g.E 
+        ==> (u in vc || v in vc) 
 }
 
 /**
@@ -45,8 +43,7 @@ The reduction: independentSet <=p vertexCover
 
 // Reduction function. This reduction is trivial.
 function indSet_to_vertexCover(g: Graph, k: nat): nat
-    requires valid_graph(g)
-    requires k <= |g.V|
+    requires valid_graph(g) && k <= |g.V|
 {
     |g.V|-k
 } 
@@ -55,24 +52,39 @@ function indSet_to_vertexCover(g: Graph, k: nat): nat
 lemma reduction_Lemma(g: Graph, k: nat)
     requires valid_graph(g)
     requires k <= |g.V|
-    ensures indSet(g, k) <==> vertexCover(g, |g.V|-k)
+    ensures indSet(g, k) <==> vertexCover(g, indSet_to_vertexCover(g, k))
 {
-    if indSet(g, k)
-    {     
-        var ins: set<nat> :| |ins| == k && ins <= g.V && is_indSet(g, ins);
-        var vc:= set u | u in g.V && u !in ins;
-        assert vc == g.V - ins;
-        assert is_vertexCover(g, vc);
-    }
-    if vertexCover(g, |g.V|-k)
-    {
-        var vc: set<nat> :| |vc| == |g.V|-k && vc <= g.V &&  is_vertexCover(g, vc);
-        var ins:=  set u | u in g.V && u !in vc;
-        assert ins == g.V - vc;
-        assert is_indSet(g, ins);
-       
-    }
+	if indSet(g, k)
+	{
+		forward_Lemma(g, k);
+	}
+	if vertexCover(g, indSet_to_vertexCover(g, k))
+	{
+		backward_Lemma(g, k);
+	}
 }
 
-// 40 code lines
+lemma forward_Lemma(g: Graph, k: nat)
+	requires valid_graph(g) && k <= |g.V|
+    requires indSet(g, k)
+	ensures vertexCover(g, |g.V|-k)
+{
+    var ins: set<nat> :| |ins| == k && ins <= g.V && is_indSet(g, ins);
+    var vc:= set u | u in g.V && u !in ins;
+    assert vc == g.V - ins;
+    assert is_vertexCover(g, vc);
+}
+
+lemma backward_Lemma (g: Graph, k: nat)
+	requires valid_graph(g) && k <= |g.V|
+    requires vertexCover(g, indSet_to_vertexCover(g, k))
+	ensures indSet(g, k)
+{
+    var vc: set<nat> :| |vc| == |g.V|-k && vc <= g.V &&  is_vertexCover(g, vc);
+    var ins:=  set u | u in g.V && u !in vc;
+    assert ins == g.V - vc;
+    assert is_indSet(g, ins);      
+}
+
+// 45 code lines
 
